Certainly, I'll format each step properly to improve clarity and readability. Here's the revised solution with better formatting:

Let's approach this step-by-step to show that for any choice of θ, there exists γ such that pθ(y|x) = pγ(y|x).

1) First, let's expand pθ(y|x) using the given formula:

   $$
   p_θ(y|x) = \frac{\pi_y \cdot \exp\left(-\frac{1}{2σ^2}(x-μ_y)^⊤(x-μ_y)\right) \cdot Z^{-1}(σ)}{\sum_i \pi_i \cdot \exp\left(-\frac{1}{2σ^2}(x-μ_i)^⊤(x-μ_i)\right) \cdot Z^{-1}(σ)}
   $$

2) We can simplify this by canceling out Z^−1(σ) from numerator and denominator:

   $$
   p_θ(y|x) = \frac{\pi_y \cdot \exp\left(-\frac{1}{2σ^2}(x-μ_y)^⊤(x-μ_y)\right)}{\sum_i \pi_i \cdot \exp\left(-\frac{1}{2σ^2}(x-μ_i)^⊤(x-μ_i)\right)}
   $$

3) Now, let's expand the quadratic term in the exponent:

   $$
   (x-μ_y)^⊤(x-μ_y) = x^⊤x - 2x^⊤μ_y + μ_y^⊤μ_y
   $$

4) Substituting this back:

   $$
   p_θ(y|x) = \frac{\pi_y \cdot \exp\left(-\frac{1}{2σ^2}(x^⊤x - 2x^⊤μ_y + μ_y^⊤μ_y)\right)}{\sum_i \pi_i \cdot \exp\left(-\frac{1}{2σ^2}(x^⊤x - 2x^⊤μ_i + μ_i^⊤μ_i)\right)}
   $$

5) The x^⊤x term appears in both numerator and denominator and can be factored out:

   $$
   p_θ(y|x) = \frac{\pi_y \cdot \exp\left(\frac{1}{σ^2}x^⊤μ_y - \frac{1}{2σ^2}μ_y^⊤μ_y\right)}{\sum_i \pi_i \cdot \exp\left(\frac{1}{σ^2}x^⊤μ_i - \frac{1}{2σ^2}μ_i^⊤μ_i\right)}
   $$

6) Now, let's compare this to the form of pγ(y|x):

   $$
   p_γ(y|x) = \frac{\exp(x^⊤w_y + b_y)}{\sum_i \exp(x^⊤w_i + b_i)}
   $$

7) For these to be equal, we need:

   $$
   w_y = \frac{1}{σ^2} · μ_y
   $$
   $$
   b_y = \ln(π_y) - \frac{1}{2σ^2} μ_y^⊤μ_y
   $$

8) With these choices, we have:

   $$
   \begin{align*}
   x^⊤w_y + b_y &= \frac{1}{σ^2} x^⊤μ_y + \ln(π_y) - \frac{1}{2σ^2} μ_y^⊤μ_y \\
                &= \ln(π_y) + \frac{1}{σ^2} x^⊤μ_y - \frac{1}{2σ^2} μ_y^⊤μ_y
   \end{align*}
   $$

9) Taking the exponential of both sides:

   $$
   \exp(x^⊤w_y + b_y) = π_y \cdot \exp\left(\frac{1}{σ^2} x^⊤μ_y - \frac{1}{2σ^2} μ_y^⊤μ_y\right)
   $$

Which is exactly the form we derived for pθ(y|x) in step 5.

Therefore, we have shown that for any choice of θ = (π1, ..., πk, μ1, ..., μk, σ), there exists γ = {w1, ..., wk, b1, ..., bk} such that pθ(y|x) = pγ(y|x), where:

$$
w_y = \frac{1}{σ^2} · μ_y
$$
$$
b_y = \ln(π_y) - \frac{1}{2σ^2} μ_y^⊤μ_y
$$

This completes the proof.



